@prefix culco: <http://w3id.org/culco#> .
@prefix rdf: <http://www.w3.org/1999/02/22-rdf-syntax-ns#> .
@prefix rdfs: <http://www.w3.org/2000/01/rdf-schema#> .
@prefix dcterms: <http://purl.org/dc/terms/> .
@prefix skosxl: <http://www.w3.org/2008/05/skos-xl#> . 
@prefix skos: <http://www.w3.org/2004/02/skos/core#> .
@prefix owl: <http://www.w3.org/2002/07/owl#> .
@prefix xsd: <http://www.w3.org/2001/XMLSchema#> .
@prefix foaf: <http://xmlns.com/foaf/0.1/> .
@prefix vann: <http://purl.org/vocab/vann/> .
@prefix bibo: <http://purl.org/ontology/bibo/> .
@prefix schema: <http://schema.org/> .

culco:ContentiousIssueScheme a owl:Ontology ;
	rdfs:subClassOf skos:ConceptScheme ;
	dcterms:title "CULCO: Concept Scheme for Words Matter Knowledge Graph"@en ;
	rdfs:label "Contentious Issues Scheme"@en ;
	dcterms:abstract 'The CULCO concept scheme is used to represent the knowlege graph of contentious terminology from the cultural sector. CULCO stands for "cultural contexts"'@en ;
	dcterms:created "2022-12-13"^^xsd:date ;
	dcterms:creator <https://orcid.org/0000-0001-9697-101X>,<https://orcid.org/0000-0002-6865-0021>,<https://orcid.org/0000-0002-7748-4715> ;
	dcterms:contributor <https://www.tropenmuseum.nl/en/about-tropenmuseum/contact> ;
	dcterms:license <https://creativecommons.org/licenses/by-sa/4.0/> ;
	rdfs:seeAlso <https://www.tropenmuseum.nl/en/about-tropenmuseum/words-matter-publication> ;
	foaf:depiction <https://github.com/cultural-ai/wordsmatter/blob/main/wm_kg_schema.png> ;
	bibo:doi "10.5281/zenodo.7456064"@en ;
	bibo:status "CULCO Scheme Specification"@en ;
	vann:namespacePrefix "culco"@en ;
	vann:namespaceURI <http://w3id.org/culco#> ;
	dcterms:replaces <http://w3id.org/culco#> ;
	owl:versionIRI <http://w3id.org/culco#> ;
	owl:versionInfo "1.0.0"@en.

<https://orcid.org/0000-0001-9697-101X> a schema:Person ;
	schema:affiliation "CWI"@en ;
	foaf:name "Andrei Nesterov"@en ;
	foaf:mbox "nesterov@cwi.nl"@en ;
	foaf:homepage <https://www.cwi.nl/people/3450> .

<https://orcid.org/0000-0002-6865-0021> a schema:Person ;
	schema:affiliation "CWI"@en ;
	foaf:name "Laura Hollink"@en ;
	foaf:mbox "l.hollink@cwi.nl"@en ;
	foaf:homepage <http://cwi.nl/~hollink> .

<https://orcid.org/0000-0002-7748-4715> a schema:Person ;
	schema:affiliation "VU University Amsterdam"@en ;
	foaf:name "Jacco van Ossenbruggen"@en ;
	foaf:mbox "jacco.van.ossenbruggen@vu.nl"@en ;
	foaf:homepage <https://research.vu.nl/en/persons/jacco-van-ossenbruggen> .

<https://www.tropenmuseum.nl/en/about-tropenmuseum/contact> a schema:Organisation ;
	schema:name "The Dutch National Museum of World Cultures"@en .

culco:ContentiousIssue a rdfs:Class;
   skos:inScheme culco:ContentiousIssueScheme ;
   rdfs:label "Contentious Issue"@en ;
   rdfs:comment "Represents a discussion about a term. In a broader sense, the discussion may have various formats and types (a textual publication, a social media post, a multimedia file, a verbal conversation etc.). A term can be a word or a phrase that causes a discussion. In the case of Words Matter, the discussion is the glossary entry, which takes one page and includes a title (a contentious term), explanations about the term's usage, and suggestions"@en .

culco:Suggestion a rdfs:Class ;
	rdfs:label "Suggestion"@en ;
	rdfs:comment "A suggestion gives recommendations on how to use a contentious term. It can be a general textual suggestion or have concrete alternatives: words and phrases to be used instead of a contentious term in specific contexts. A suggestion can refer to multiple contentious terms. Usually, a Suggestion is a part of a Contentious Issue"@en .

culco:hasSuggestion a rdf:Property ;
						rdfs:domain culco:ContentiousIssue ;
						rdfs:range culco:Suggestion ;
						rdfs:label "hasSuggestion"@en ;
						rdfs:comment "Used to link Contentious Issue to a Suggestion. Contentious Issue may have several Suggestions"@en. 

culco:hasContentiousLabel a rdf:Property ;
						rdfs:domain culco:ContentiousIssue ;
						rdfs:range skosxl:Label ;
						rdfs:label "hasContentiousLabel"@en ;
						rdfs:comment "Used to link Contentious Issue to the contentious label(s) it mentions. Technically, Suggestion may also mention contentious labels"@en .

culco:hasSuggestedLabel a rdf:Property ;
						rdfs:domain culco:Suggestion ;
						rdfs:range skosxl:Label ;
						rdfs:label "hasSuggestedLabel"@en ;
						rdfs:comment "Used to link Suggestion to the suggested label(s) it mentions."@en .

culco:suggestedFor a rdf:Property ;
						rdfs:domain culco:Suggestion ;
						rdfs:range skosxl:Label ;
						rdfs:label "suggestedFor"@en ;
						rdfs:comment "Used to link Suggestion to the contentious label(s) it is suggested for."@en .
	
culco:hasAltLabelExample a rdf:Property ;
						rdfs:domain culco:Suggestion ;
						rdfs:range skosxl:Label ;
						rdfs:label "hasAltLabelExample"@en ;
						rdfs:comment "Used with Suggestions when a suggestion gives an example of a contextually appropriate synonym, but not a complete alternative to a contentious label. For example,  the term 'Moroccan-Dutch' is one of the possible alternatives for the contentious term 'Allochtoon'"@en .

culco:hasUsageExample a rdf:Property  ;
						rdfs:domain culco:Suggestion ;
						rdfs:range xsd:string ;
						rdfs:label "hasUsageExample"@en ;
						rdfs:comment "Used with Suggestions when it gives an example of how a contentious term or its synonym can be used appropriately in speech; usually, it is a phrase providing additional context in which it is appropriate to use the mentioned terms, for example, the phrase 'There was an artistic movement called ‘primitivism’ for the term 'Primitive'"@en .
