@prefix culco: <https://w3id.org/culco> .
@prefix rdf: <http://www.w3.org/1999/02/22-rdf-syntax-ns#> .
@prefix rdfs: <https://www.w3.org/2000/01/rdf-schema> .
@prefix dcterms: <http://purl.org/dc/terms/> .
@prefix skosxl: <http://www.w3.org/2008/05/skos-xl#> . 
@prefix skos: <http://www.w3.org/2004/02/skos/core#> .

culco:ContentiousIssueScheme rdfs:subClassOf skos:ConceptScheme ;
dcterms:title "Concept Scheme for Words Matter Knowledge Graph"@en .

culco:ContentiousIssue a rdfs:Class ;
   skos:inScheme culco:ContentiousIssueScheme ;
   rdfs:label "Contentious Issue"@en ;
   rdfs:comment "Represents a discussion about a term. In a broader sense, the discussion may have various formats and types (a textual publication, a social media post, a multimedia file, a verbal conversation etc.). A term can be a word or a phrase that causes a discussion. In the case of Words Matter, the discussion is the glossary entry, which takes one page and includes a title (a contentious term), explanations about the term's usage, and suggestions"@en .

culco:Suggestion a rdfs:Class ;
	rdfs:label "Suggestion"@en ;
	rdfs:comment "A suggestion gives recommendations on how to use a contentious term. It can be a general textual suggestion or have concrete alternatives: words and phrases to be used instead of a contentious term in specific contexts. A suggestion can refer to multiple contentious terms. Usually, a Suggestion is a part of a Contentious Issue"@en .

culco:hasSuggestion a rdf:Property ;
						rdfs:domain culco:ContentiousIssue ;
						rdfs:range culco:Suggestion ;
						rdfs:label "hasSuggestion"@en ;
						rdfs:comment "Used to link Contentious Issue to a Suggestion. Contentious Issue may have several Suggestions"@en. 

culco:hasContentiousLabel a rdf:Property ;
						rdfs:range skosxl:Label ;
						rdfs:label "hasContentiousLabel"@en ;
						rdfs:comment "Used to link Contentious Issue to the contentious label(s) it mentions. Technically, Suggestion may also mention contentious labels"@en .

culco:hasSuggestedLabel a rdf:Property ;
						rdfs:domain culco:Suggestion ;
						rdfs:range skosxl:Label ;
						rdfs:label "hasSuggestedLabel"@en ;
						rdfs:comment "Used to link Suggestion to the suggested label(s) it mentions."@en .

culco:suggestedFor a rdf:property ;
						rdfs:domain culco:Suggestion ;
						rdfs:range skosxl:Label ;
						rdfs:label "suggestedFor"@en ;
						rdfs:comment "Used to link Suggestion to the contentious label(s) it is suggested for."@en .
	
culco:hasAltLabelExample a rdf:Property ;
						rdfs:domain culco:Suggestion ;
						rdfs:label "hasAltLabelExample"@en ;
						rdfs:comment "Used with Suggestions when a suggestion gives an example of a contextually appropriate synonym, but not a complete alternative to a contentious label. For example,  the term 'Moroccan-Dutch' is one of the possible alternatives for the contentious term 'Allochtoon'"@en .

culco:hasUsageExample a rdf:Property  ;
						rdfs:domain culco:Suggestion ;
						rdfs:label "hasUsageExample"@en ;
						rdfs:comment "Used with Suggestions when it gives an example of how a contentious term or its synonym can be used appropriately in speech; usually, it is a phrase providing additional context in which it is appropriate to use the mentioned terms, for example, the phrase 'There was an artistic movement called ‘primitivism’ for the term 'Primitive'"@en .